Examples/runtimes/java/DynamoDbEncryption/build.gradle.kts
@@ -38,12 +38,12 @@ if (!caPasswordString.isNullOrBlank()) {
 }
 
 repositories {
+    mavenLocal()
     maven {
         name = "DynamoDB Local Release Repository - US West (Oregon) Region"
         url  = URI.create("https://s3-us-west-2.amazonaws.com/dynamodb-local/release")
     }
     mavenCentral()
-    mavenLocal()
     if (caUrl != null && caPassword != null) {
         maven {
             name = "CodeArtifact"
